@prefix : <http://lod.unige.ch/segmOnto/> .
@prefix owl: <http://www.w3.org/2002/07/owl#> .
@prefix rdf: <http://www.w3.org/1999/02/22-rdf-syntax-ns#> .
@prefix xml: <http://www.w3.org/XML/1998/namespace> .
@prefix xsd: <http://www.w3.org/2001/XMLSchema#> .
@prefix rdfs: <http://www.w3.org/2000/01/rdf-schema#> .
@prefix vann: <http://purl.org/vocab/vann/> .
@base <http://lod.unige.ch/segmOnto/> .

<http://lod.unige.ch/segmOnto/>     rdf:type owl:Ontology ;
                                    owl:imports <https://cidoc-crm.org/rdfs/7.1.1/CIDOC_CRM_v7.1.1.rdfs> ;
                                    vann:preferredNamespacePrefix "sgm" ;
                                    vann:preferredNamespaceUri "http://lod.unige.ch/segmOnto/" .


:Line rdf:type owl:Class ;
      rdfs:subClassOf :Textual_Body ;
      rdfs:comment "Lines are rows of physically continuous text which are spatially discontinued from other element of the page"@en ;
      rdfs:label "Line"@en .



:Textual_Body rdf:type owl:Class ;
              rdfs:subClassOf <http://www.cidoc-crm.org/cidoc-crm/E25_Human-Made_Feature> ;
              rdfs:comment "The Textual Body is a delimited space carrying text. The nature of a Textual body is physical and it expresses how the text can be accessed and viewed.  We do not differentiate a \"Textual Body\" by their physical material support, and the class can be used to document handwritten, typed, printed texts as well as any other material support (for example, an epigraph) which is used to contain a textual source."@en ;
              rdfs:label "Textual Body"@en .



:Zone rdf:type owl:Class ;
      rdfs:subClassOf :Textual_Body ;
      rdfs:comment "Zones are portion (segments) of the Textual Body. The identity of a Zone corresponds to the boundaries of a subsection on the Textual Body as recognised by a human or a computational process. The aim of a zone is to identify, delimit and classify portions of a Textual Body that tells us about the organization and type of information present on the medium."@en ;
      rdfs:label "Zone"@en .


